\section{Structural equality}

\begin{frame}[fragile]{Specification}
\large
\begin{minted}{coq}
Axiom structeq_spec : ∀ `{zoo_G : !ZooG Σ} {v1 v2} footprint,
  val_traversable footprint v1 →
  val_traversable footprint v2 →
  {{{
    structeq_footprint footprint
  }}}
    v1 = v2
  {{{ b,
    RET #b;
    structeq_footprint footprint ∗
    ⌜(if b then val_structeq else val_structneq) footprint v1 v2⌝
  }}}.
\end{minted}
\end{frame}

\begin{frame}[fragile]{Specification for \emph{abstract} values}
\large
\begin{minted}{coq}
Lemma structeq_spec_abstract `{zoo_G : !ZooG Σ} v1 v2 :
  val_abstract v1 →
  val_abstract v2 →
  {{{
    True
  }}}
    v1 = v2
  {{{ b,
    RET #b;
    ⌜(if b then (≈) else (≉)) v1 v2⌝
  }}}
Proof.
  ...
Qed.
\end{minted}
\end{frame}